Nickelean.lean
@@ -10,3 +10,5 @@ import Nickelean.Float64
 import Nickelean.RecordOrder
 import Nickelean.Tests
 import Nickelean.DecidableEq
+import Nickelean.PrintJson
+import Nickelean.CrossValidation
